reduction draft

Core/Term/Spine.lean
@@ -1,18 +1,38 @@
 import LeanSubst
 import Core.Term.Definition
+import Core.Term.Beq
 
 open LeanSubst
 
 inductive SpineElem : Type where
 | type (x : Ty)
 | term (x : Term)
+| oterm (x : Term)
+
+def SpineElem.beq : SpineElem -> SpineElem -> Bool
+| type A, type B => A == B
+| term a, term b => a == b
+| oterm a, oterm b => a == b
+| _, _ => false
+
+instance : BEq SpineElem where
+  beq := SpineElem.beq
 
 def Term.spine : Term -> Option (String × List SpineElem)
 | g#x => return (x, [])
 | ctor2 .app f a => do
   let (x, sp) <- spine f
   (x, sp ++ [.term a])
+| f ∘[a] => do
+  let (x, sp) <- spine f
+  (x, sp ++ [.oterm a])
 | f •[a] => do
   let (x, sp) <- spine f
   (x, sp ++ [.type a])
 | _ => none
+
+def Term.apply (t : Term) : List SpineElem -> Term
+| [] => t
+| .cons (.type A) tl => (t •[A]).apply tl
+| .cons (.term a) tl => (t • a).apply tl
+| .cons (.oterm a) tl => (t ∘[a]).apply tl
