Core/Global.lean
@@ -23,13 +23,14 @@ def lookup_kind (x : String) : List Global -> Option Kind
 def lookup_type (x : String) : List Global -> Option Ty
 | [] => none
 | .cons (.data _ _ ctors) t =>
-
   sorry
 | .cons (.openm n A) t
 | .cons (.let n A _) t
 | .cons (.instty n A) t =>
   if n == x then A else lookup_type x t
 | .cons _ t => lookup_type x t
+
+def instances (x : String) : List Global -> Option (List Term) := sorry
 
 def is_ctor : List Global -> String -> Bool := sorry
 
@@ -38,3 +39,9 @@ def is_datatype : List Global -> String -> Bool := sorry
 def is_instty : List Global -> String -> Bool := sorry
 
 def is_opent : List Global -> String -> Bool := sorry
+
+def is_openm : List Global -> String -> Bool := sorry
+
+def ctor_idx : List Global -> String -> Option (Fin n) := sorry
+
+def is_stable : List Global -> String -> Bool := sorry
