Core/Reduction.lean
@@ -1,0 +1,159 @@
+import LeanSubst
+import Core.Util
+import Core.Global
+import Core.Ty
+import Core.Term
+
+open LeanSubst
+
+def OpenVarVal (G : List Global) (x : String) (sp : List SpineElem) : Prop :=
+  is_openm G x ∧ ∀ T, some T = lookup_type x G -> sp.length < T.arity
+
+inductive Value (G : List Global) : Term -> Prop where
+| app :
+  some (x, sp) = t.spine ->
+  is_stable G x ∨ OpenVarVal G x sp ->
+  Value G t
+| choice : Value G t1 -> Value G t2 -> Value G (t1 `+ t2)
+| lam : Value G (λ[A] t)
+| lamt : Value G (Λ[K] t)
+| refl : Value G (refl! A)
+
+def Ctor2Variant.congr1 : Ctor2Variant -> Bool
+| app => true
+| appo => true
+| cast => false
+| seq => true
+| appc => true
+| apptc => true
+| arrowc => true
+| choice => true
+
+def Ctor2Variant.congr2 : Ctor2Variant -> Bool
+| app => false
+| appo => false
+| cast => true
+| seq => true
+| appc => true
+| apptc => true
+| arrowc => true
+| choice => true
+
+def TyBindVariant.congr : TyBindVariant -> Bool
+| lamt => false
+| allc => true
+
+inductive Red (G : List Global) : Term -> Term -> Prop where
+----------------------------------------------------------------
+---- Basic Reduction Steps
+----------------------------------------------------------------
+| beta : Red G ((λ[A] b) • t) b[su t::+0]
+| betat : Red G ((Λ[A] b) •[t]) b[su t::+0:Ty]
+| cast : Red G (t ▹ refl! A) t
+| sym : Red G (sym! (refl! A)) (refl! A)
+| seq : Red G ((refl! A) `; (refl! A)) (refl! A)
+| appc : Red G ((refl! A) •c (refl! B)) (refl! (A • B))
+| apptc : Red G ((refl! (∀[K] A)) •c[refl! B]) (refl! A[su B::+0])
+| fst : Red G (fst! (refl! (A • B))) (refl! A)
+| snd : Red G (snd! (refl! (A • B))) (refl! B)
+| allc : Red G (∀c[A] refl! B) (refl! (∀[A] B))
+| arrowc : Red G ((refl! A) -c> (refl! B)) (refl! (A -:> B))
+| choice1 : Red G (`0 `+ t) t
+| choice2 : Red G (t `+ `0) t
+----------------------------------------------------------------
+---- Data Matching
+----------------------------------------------------------------
+| data_match {i : Fin n} :
+  some (x, sp) = Term.spine p ->
+  some (x, sp') = Term.spine s ->
+  some q = prefix_equal sp sp' ->
+  some i = ctor_idx G x ->
+  Red G (.match p s cs) ((cs i).apply q)
+----------------------------------------------------------------
+---- Guard Matching
+----------------------------------------------------------------
+| guard_matched :
+  some (x, sp) = Term.spine p ->
+  some (x, sp') = Term.spine s ->
+  some q = prefix_equal sp sp' ->
+  Red G (.guard p s b) (b.apply q)
+| guard_missed :
+  some (x, sp) = Term.spine p ->
+  some (x', sp') = Term.spine s ->
+  x ≠ x' ∨ none = prefix_equal sp sp' ->
+  Red G (.guard p s b) `0
+----------------------------------------------------------------
+---- Instance Instantiation
+----------------------------------------------------------------
+| inst :
+  some (x, sp) = Term.spine h ->
+  (∀ e ∈ sp, ∀ a, .oterm a = e -> Value G a) ->
+  some T = lookup_type x G ->
+  sp.length ≥ T.arity ->
+  some tl = instances x G ->
+  tl' = List.map (·.apply sp) tl ->
+  h' = List.foldl (·`+·) `0 tl' ->
+  Red G h h'
+----------------------------------------------------------------
+---- Congruence Rules
+----------------------------------------------------------------
+| ctor1_congr :
+  Red G t t' ->
+  Red G (.ctor1 v t) (.ctor1 v t')
+| ctor2_congr1 :
+  v.congr1 ->
+  Red G t1 t1' ->
+  Red G (.ctor2 v t1 t2) (.ctor2 v t1' t2)
+| ctor2_congr2 :
+  v.congr2 ->
+  Red G t2 t2' ->
+  Red G (.ctor2 v t1 t2) (.ctor2 v t1 t2')
+| tbind_congr :
+  v.congr ->
+  Red G t t' ->
+  Red G (.tbind v K t) (.tbind v K t')
+| guard_congr :
+  Red G s s' ->
+  Red G (.guard p s b) (.guard p s' b)
+| match_congr :
+  Red G s s' ->
+  Red G (.match p s ts) (.match p s' ts)
+----------------------------------------------------------------
+---- Absorption Rules
+----------------------------------------------------------------
+| ctor1_asborb :
+  Red G (.ctor1 v `0) `0
+| ctor2_asborb1 :
+  v.congr1 ->
+  Red G (.ctor2 v `0 t2) `0
+| ctor2_asborb2 :
+  v.congr2 ->
+  Red G (.ctor2 v t1 `0) `0
+| tbind_asborb :
+  v.congr ->
+  Red G (.tbind v K `0) `0
+| guard_asborb :
+  Red G (.guard p `0 b) `0
+| match_asborb :
+  Red G (.match p `0 ts) `0
+----------------------------------------------------------------
+---- Mapping Rules
+----------------------------------------------------------------
+| ctor1_map :
+  Red G t t' ->
+  Red G (.ctor1 v (c1 `+ c2)) (.ctor1 v c1 `+ .ctor1 v c2)
+| ctor2_map1 :
+  v.congr1 ->
+  v ≠ .choice ->
+  Red G (.ctor2 v (c1 `+ c2) t2) (.ctor2 v c1 t2 `+ .ctor2 v c2 t2)
+| ctor2_map2 :
+  v.congr2 ->
+  v ≠ .choice ->
+  Red G (.ctor2 v t1 (c1 `+ c2)) (.ctor2 v t1 c1 `+ .ctor2 v t1 c2)
+| tbind_map :
+  v.congr ->
+  Red G (.tbind v K (c1 `+ c2)) (.tbind v K c1 `+ .tbind v K c2)
+| guard_map :
+  Red G (.guard p (c1 `+ c2) b) (.guard p c1 b `+ .guard p c2 b)
+| match_map :
+  Red G (.match p (c1 `+ c2) ts) (.match p c1 ts `+ .match p c2 ts)
