Core/Term/BEq.lean
@@ -1,0 +1,61 @@
+import Core.Ty
+import Core.Term.Definition
+
+def Ctor0Variant.beq : Ctor0Variant -> Ctor0Variant -> Bool
+| zero, zero => true
+| refl A, refl B => A == B
+| _, _ => false
+
+instance : BEq Ctor0Variant where
+  beq := Ctor0Variant.beq
+
+def Ctor1Variant.beq : Ctor1Variant -> Ctor1Variant -> Bool
+| sym, sym => true
+| fst, fst => true
+| snd, snd => true
+| appt a, appt b => a == b
+| _, _ => false
+
+instance : BEq Ctor1Variant where
+  beq := Ctor1Variant.beq
+
+def Ctor2Variant.beq : Ctor2Variant -> Ctor2Variant -> Bool
+| app, app => true
+| appo, appo => true
+| cast, cast => true
+| seq, seq => true
+| appc, appc => true
+| apptc, apptc => true
+| arrowc, arrowc => true
+| choice, choice => true
+| _, _ => false
+
+instance : BEq Ctor2Variant where
+  beq := Ctor2Variant.beq
+
+def TyBindVariant.beq : TyBindVariant -> TyBindVariant -> Bool
+| lamt, lamt => true
+| allc, allc => true
+| _, _ => false
+
+instance : BEq TyBindVariant where
+  beq := TyBindVariant.beq
+
+def Term.beq : Term -> Term -> Bool
+| var x, var y => x == y
+| global x, global y => x == y
+| ctor0 c1, ctor0 c2 => c1 == c2
+| ctor1 c1 a1, ctor1 c2 a2 => c1 == c2 && beq a1 a2
+| ctor2 c1 a1 b1, ctor2 c2 a2 b2 => c1 == c2 && beq a1 a2 && beq b1 b2
+| tbind A1 K1 t1, tbind A2 K2 t2 => A1 == A2 && K1 == K2 && beq t1 t2
+| lam A1 t1, lam A2 t2 => A1 == A2 && beq t1 t2
+| guard a1 b1 c1, guard a2 b2 c2 => beq a1 a2 && beq b1 b2 && beq c1 c2
+| .match (n := n1) a1 b1 c1, .match (n := n2) a2 b2 c2 =>
+  if h : n1 = n2 then
+    let c : Vec Bool n1 := λ i => beq (c1 i) (c2 (by rw [h] at i; exact i))
+    beq a1 a2 && beq b1 b2 && Vec.fold (·&&·) true c
+  else false
+| _, _ => false
+
+instance : BEq Term where
+  beq := Term.beq
