Core/Term/Definition.lean
@@ -60,7 +60,7 @@ notation t1 " `; " t2 => Term.ctor2 Ctor2Variant.seq t1 t2
 notation f " •c " a => Term.ctor2 Ctor2Variant.appc f a
 notation f " •c[" a "]" => Term.ctor2 Ctor2Variant.apptc f a
 notation A " -c> " B => Term.ctor2 Ctor2Variant.arrowc A B
-notation t1 " + " t2 => Term.ctor2 Ctor2Variant.choice t1 t2
+notation t1 " `+ " t2 => Term.ctor2 Ctor2Variant.choice t1 t2
 
 -- bind notation
 notation "Λ[" K "]" t => Term.tbind TyBindVariant.lamt K t
@@ -68,3 +68,15 @@ notation "λ[" A "]" t => Term.lam A t
 notation "∀c[" K "]" P => Term.tbind TyBindVariant.allc K P
 
 notation "match!" => Term.match
+
+@[simp]
+def Term.size : Term -> Nat
+| var _ => 0
+| global _ => 0
+| ctor0 _ => 0
+| ctor1 _ t => size t + 1
+| ctor2 _ t1 t2 => size t1 + size t2 + 1
+| tbind _ _ t => size t + 1
+| lam _ t => size t + 1
+| guard t1 t2 t3 => size t1 + size t2 + size t3 + 1
+| .match t1 t2 ts => size t1 + size t2 + Vec.sum (λ i => (ts i).size) + 1
