Core/Ty.lean
@@ -1,3 +1,4 @@
 import Core.Ty.Definition
+import Core.Ty.BEq
 import Core.Ty.Substitution
-import Core.Ty.Spine
+import Core.Ty.Structure
