Core/Ty/BEq.lean
@@ -1,0 +1,29 @@
+import Core.Ty.Definition
+
+def BaseKind.beq : BaseKind -> BaseKind -> Bool
+| .open, .open => true
+| closed, closed => true
+| _, _ => false
+
+instance : BEq BaseKind where
+  beq := BaseKind.beq
+
+def Kind.beq : Kind -> Kind -> Bool
+| base b1, base b2 => b1 == b2
+| arrow A1 B1, arrow A2 B2 => beq A1 A2 && beq B1 B2
+| _, _ => false
+
+instance : BEq Kind where
+  beq := Kind.beq
+
+def Ty.beq : Ty -> Ty -> Bool
+| var x, var y => x == y
+| global x, global y => x == y
+| arrow A1 B1, arrow A2 B2 => beq A1 A2 && beq B1 B2
+| all K1 P1, all K2 P2 => K1 == K2 && beq P1 P2
+| app A1 B1, app A2 B2 => beq A1 A2 && beq B1 B2
+| eq K1 A1 B1, eq K2 A2 B2 => K1 == K2 && beq A1 A2 && beq B1 B2
+| _, _ => false
+
+instance : BEq Ty where
+  beq := Ty.beq
