Core/Util.lean
@@ -1,0 +1,40 @@
+
+@[simp]
+def prefix_equal [BEq T] : List T -> List T -> Option (List T)
+| [], t => .some t
+| .cons _ _, [] => .none
+| .cons x1 t1, .cons x2 t2 => if x1 == x2 then prefix_equal t1 t2 else .none
+
+theorem prefix_equal_law [BEq T] [LawfulBEq T] {p t1 t2 : List T}
+  : .some p = prefix_equal t1 t2 -> t2 = t1 ++ p
+:= by
+intro h
+induction t1, t2 using prefix_equal.induct generalizing p
+case _ => simp at h; subst h; simp
+case _ => simp at h
+case _ h2 ih =>
+    replace h2 := LawfulBEq.eq_of_beq h2; subst h2
+    simp at h; rw [ih h]; simp
+case _ h2 =>
+  simp at *; exfalso
+  apply h2; apply h.1
+
+instance : Monad List where
+  pure a := List.cons a List.nil
+  bind l f := List.flatten (List.map f l)
+
+theorem option_lemma :
+  (∀ v, ¬ t = Option.some v) ->
+  t = .none
+:= by
+intro h
+cases t; simp
+case _ v => exfalso; apply h v rfl
+
+theorem not_eq_of_beq [BEq T] [LawfulBEq T] {x y : T} : ¬ ((x == y) = true) -> x ≠ y := by
+intro h1 h2; subst h2; apply h1; simp
+
+@[simp]
+def rep (f : T -> T) (x : T) : Nat -> T
+| 0 => x
+| n + 1 => f (rep f x n)
